revm: simulate: more work

RocqOfRust/revm/revm_interpreter/instructions/simulate/memory/msize.v
@@ -1,54 +1,73 @@
 Require Import simulate.RocqOfRust.
-Require Import alloy_primitives.bytes.simulate.mod.
 Require Import alloy_primitives.links.aliases.
 Require Import core.links.array.
+Require Import core.ops.simulate.deref.
+Require Import core.simulate.option.
+Require Import revm.revm_context_interface.links.host.
 Require Import revm.revm_interpreter.gas.simulate.constants.
-Require Import revm.revm_interpreter.instructions.links.control.jumpdest_or_nop.
 Require Import revm.revm_interpreter.instructions.simulate.macros.
+Require Import revm.revm_interpreter.interpreter.simulate.shared_memory.
 Require Import revm.revm_interpreter.links.gas.
-Require Import revm.revm_interpreter.links.instruction_result.
 Require Import revm.revm_interpreter.links.interpreter.
-Require Import revm.revm_interpreter.links.interpreter_action.
 Require Import revm.revm_interpreter.links.interpreter_types.
+Require Import revm.revm_interpreter.simulate.gas.
 Require Import revm.revm_interpreter.simulate.interpreter_types.
 Require Import revm.revm_specification.links.hardfork.
 Require Import revm.revm_specification.simulate.hardfork.
 Require Import ruint.links.lib.
-Require Import ruint.simulate.cmp.
+Require Import ruint.simulate.bytes.
 Require Import ruint.simulate.from.
-Require Import ruint.simulate.lib.
 
-Definition jumpdest_or_nop
+Require Import revm.revm_interpreter.instructions.links.memory.msize.
+
+Definition msize
     {WIRE : Set} `{Link WIRE}
     {WIRE_types : InterpreterTypes.Types.t} `{InterpreterTypes.Types.AreLinks WIRE_types}
-    {IInterpreterTypes : InterpreterTypes.C WIRE_types}
+    `{!InterpreterTypes.C WIRE_types}
     (interpreter : Interpreter.t WIRE WIRE_types) :
     Interpreter.t WIRE WIRE_types :=
-  gas_macro interpreter constants.JUMPDEST id (fun interpreter => interpreter).
+  gas_macro interpreter constants.BASE id (fun interpreter =>
+    let IInterpreterTypes := _ in
+    let size :=
+      IInterpreterTypes.(InterpreterTypes.MemoryTrait_for_Memory).(MemoryTrait.size)
+        interpreter.(Interpreter.memory) in
+    let value : aliases.U256.t := {| Uint.value := i[size] |} in
+    push_macro interpreter value id (fun interpreter => interpreter)).
 
-Lemma jumpdest_or_nop_eq
+Lemma msize_eq
     {WIRE H : Set} `{Link WIRE} `{Link H}
     {WIRE_types : InterpreterTypes.Types.t} `{InterpreterTypes.Types.AreLinks WIRE_types}
+    {H_types : Host.Types.t} `{Host.Types.AreLinks H_types}
     (run_InterpreterTypes_for_WIRE : InterpreterTypes.Run WIRE WIRE_types)
     (IInterpreterTypes : InterpreterTypes.C WIRE_types)
     (InterpreterTypesEq :
       InterpreterTypes.Eq.t WIRE WIRE_types run_InterpreterTypes_for_WIRE IInterpreterTypes)
     (interpreter : Interpreter.t WIRE WIRE_types)
     (_host : H) :
-  let ref_interpreter := make_ref 0 in
-  let ref_host := make_ref (A := H) 1 in
+  let ref_interpreter : '&mut (Interpreter.t WIRE WIRE_types) := make_ref 0 in
+  let ref_host : '&mut H := make_ref 1 in
   {{
     SimulateM.eval_f
-      (run_jumpdest_or_nop run_InterpreterTypes_for_WIRE ref_interpreter ref_host)
+      (run_msize run_InterpreterTypes_for_WIRE ref_interpreter ref_host)
       ([interpreter; _host]%stack) 🌲
     (
       Output.Success tt,
-      [jumpdest_or_nop interpreter; _host]%stack
+      [
+        msize interpreter;
+        _host
+      ]%stack
     )
   }}.
 Proof.
   intros.
-  with_strategy transparent [run_jumpdest_or_nop] unfold jumpdest_or_nop, run_jumpdest_or_nop; cbn.
+  unfold msize.
   gas_macro_eq InterpreterTypesEq.
+  s. {
+    apply InterpreterTypesEq.
+  }
+  s. {
+    s_apply Impl_Uint.from_eq.
+  }
+  push_macro_eq InterpreterTypesEq.
   s.
 Qed.
