RocqOfRust/ruint/simulate/div.v
@@ -19,4 +19,21 @@ Module Impl_Uint.
       )
     }}.
   Admitted.
+  Definition wrapping_rem {BITS LIMBS : usize} (x1 x2 : lib.Uint.t BITS LIMBS) :
+      lib.Uint.t BITS LIMBS :=
+    {| lib.Uint.value := x1.(lib.Uint.value) mod x2.(lib.Uint.value) |}.
+
+  Lemma wrapping_rem_eq
+      (stack : Stack.t)
+      (BITS LIMBS : usize) (x1 x2 : lib.Uint.t BITS LIMBS) :
+    {{
+      SimulateM.eval_f
+        (Impl_Uint.run_wrapping_rem BITS LIMBS x1 x2)
+        stack 🌲
+      (
+        Output.Success (wrapping_rem x1 x2),
+        stack
+      )
+    }}.
+  Admitted.
 End Impl_Uint.
