RocqOfRust/revm/revm_interpreter/instructions/simulate/memory/mcopy.v
@@ -1,0 +1,75 @@
+Require Import simulate.RocqOfRust.
+Require Import alloy_primitives.links.aliases.
+Require Import core.links.array.
+Require Import core.ops.simulate.deref.
+Require Import core.simulate.option.
+Require Import revm.revm_context_interface.links.host.
+Require Import revm.revm_interpreter.gas.simulate.constants.
+Require Import revm.revm_interpreter.instructions.simulate.macros.
+Require Import revm.revm_interpreter.interpreter.simulate.shared_memory.
+Require Import revm.revm_interpreter.links.gas.
+Require Import revm.revm_interpreter.links.interpreter.
+Require Import revm.revm_interpreter.links.interpreter_types.
+Require Import revm.revm_interpreter.simulate.gas.
+Require Import revm.revm_interpreter.simulate.interpreter_types.
+Require Import revm.revm_specification.links.hardfork.
+Require Import revm.revm_specification.simulate.hardfork.
+Require Import ruint.links.lib.
+Require Import ruint.simulate.bytes.
+Require Import ruint.simulate.from.
+
+Require Import revm.revm_interpreter.instructions.links.memory.mcopy.
+
+Definition mcopy
+    {WIRE : Set} `{Link WIRE}
+    {WIRE_types : InterpreterTypes.Types.t} `{InterpreterTypes.Types.AreLinks WIRE_types}
+    `{!InterpreterTypes.C WIRE_types}
+    (interpreter : Interpreter.t WIRE WIRE_types) :
+    Interpreter.t WIRE WIRE_types :=
+  check_macro interpreter SpecId.CANCUN id (fun interpreter =>
+  popn_macro interpreter {| Integer.value := 3 |} id (fun arr interpreter =>
+    let '⟬ dst_u256; src_u256; len_u256 ⟭ := arr.(array.value) in
+    as_usize_or_fail_ret_macro interpreter len_u256 None id (fun len interpreter =>
+      if i[len] =? 0 then
+        interpreter
+      else
+        as_usize_or_fail_ret_macro interpreter dst_u256 None id (fun dst interpreter =>
+        as_usize_or_fail_ret_macro interpreter src_u256 None id (fun src interpreter =>
+          let words_num := num_words len in
+          let copy_cost : u64 := {| Integer.value := i[constants.VERYLOW] + i[words_num] * i[constants.COPY] |} in
+          gas_macro interpreter copy_cost id (fun interpreter =>
+            let max_offset : usize := {| Integer.value := Z.max i[dst] i[src] |} in
+            resize_memory_macro interpreter max_offset len id (fun interpreter =>
+              let IInterpreterTypes := _ in
+              let memory :=
+                IInterpreterTypes.(InterpreterTypes.MemoryTrait_for_Memory).(MemoryTrait.copy)
+                  interpreter.(Interpreter.memory) dst src len in
+              interpreter <| Interpreter.memory := memory |>
+            ))))))).
+
+Lemma mcopy_eq
+    {WIRE H : Set} `{Link WIRE} `{Link H}
+    {WIRE_types : InterpreterTypes.Types.t} `{InterpreterTypes.Types.AreLinks WIRE_types}
+    {H_types : Host.Types.t} `{Host.Types.AreLinks H_types}
+    (run_InterpreterTypes_for_WIRE : InterpreterTypes.Run WIRE WIRE_types)
+    (IInterpreterTypes : InterpreterTypes.C WIRE_types)
+    (InterpreterTypesEq :
+      InterpreterTypes.Eq.t WIRE WIRE_types run_InterpreterTypes_for_WIRE IInterpreterTypes)
+    (interpreter : Interpreter.t WIRE WIRE_types)
+    (_host : H) :
+  let ref_interpreter : '&mut (Interpreter.t WIRE WIRE_types) := make_ref 0 in
+  let ref_host : '&mut H := make_ref 1 in
+  {{
+    SimulateM.eval_f
+      (run_mcopy run_InterpreterTypes_for_WIRE ref_interpreter ref_host)
+      ([interpreter; _host]%stack) 🌲
+    (
+      Output.Success tt,
+      [
+        mcopy interpreter;
+        _host
+      ]%stack
+    )
+  }}.
+Proof.
+Admitted.
