RocqOfRust/revm/revm_interpreter/instructions/simulate/memory/mload.v
@@ -1,0 +1,92 @@
+Require Import simulate.RocqOfRust.
+Require Import alloy_primitives.links.aliases.
+Require Import core.links.array.
+Require Import core.ops.simulate.deref.
+Require Import core.simulate.option.
+Require Import revm.revm_context_interface.links.host.
+Require Import revm.revm_interpreter.gas.simulate.constants.
+Require Import revm.revm_interpreter.instructions.simulate.macros.
+Require Import revm.revm_interpreter.interpreter.simulate.shared_memory.
+Require Import revm.revm_interpreter.links.gas.
+Require Import revm.revm_interpreter.links.interpreter.
+Require Import revm.revm_interpreter.links.interpreter_types.
+Require Import revm.revm_interpreter.simulate.gas.
+Require Import revm.revm_interpreter.simulate.interpreter_types.
+Require Import revm.revm_specification.links.hardfork.
+Require Import revm.revm_specification.simulate.hardfork.
+Require Import ruint.links.lib.
+Require Import ruint.simulate.bytes.
+Require Import ruint.simulate.from.
+
+Require Import revm.revm_interpreter.instructions.links.memory.mload.
+
+Definition mload
+    {WIRE : Set} `{Link WIRE}
+    {WIRE_types : InterpreterTypes.Types.t} `{InterpreterTypes.Types.AreLinks WIRE_types}
+    `{!InterpreterTypes.C WIRE_types}
+    (interpreter : Interpreter.t WIRE WIRE_types) :
+    Interpreter.t WIRE WIRE_types :=
+  gas_macro interpreter constants.VERYLOW id (fun interpreter =>
+  popn_top_macro interpreter 0 id (fun _ top interpreter =>
+  let top := top.(RefStub.projection) interpreter.(Interpreter.stack) in
+  as_usize_or_fail_macro interpreter top None id (fun offset interpreter =>
+  resize_memory_macro interpreter offset 32 id (fun interpreter =>
+      (* let IInterpreterTypes := _ in
+      let memory_synthetic :=
+        IInterpreterTypes.(InterpreterTypes.MemoryTrait_for_Memory).(MemoryTrait.slice_len)
+          interpreter.(Interpreter.memory) offset 32 in
+      let deref_stub :=
+        IInterpreterTypes.(InterpreterTypes.MemoryTrait_for_Memory).(MemoryTrait.Deref_for_Synthetic1).(Deref.deref) in
+      let bytes := deref_stub.(RefStub.projection) memory_synthetic in
+      let value := u256_from_be_bytes bytes in
+      let stack := top.(RefStub.injection) interpreter.(Interpreter.stack) value in
+      interpreter <| Interpreter.stack := stack |> *)
+    interpreter
+    )))).
+
+Lemma mload_eq
+    {WIRE H : Set} `{Link WIRE} `{Link H}
+    {WIRE_types : InterpreterTypes.Types.t} `{InterpreterTypes.Types.AreLinks WIRE_types}
+    {H_types : Host.Types.t} `{Host.Types.AreLinks H_types}
+    (run_InterpreterTypes_for_WIRE : InterpreterTypes.Run WIRE WIRE_types)
+    (IInterpreterTypes : InterpreterTypes.C WIRE_types)
+    (InterpreterTypesEq :
+      InterpreterTypes.Eq.t WIRE WIRE_types run_InterpreterTypes_for_WIRE IInterpreterTypes)
+    (interpreter : Interpreter.t WIRE WIRE_types)
+    (_host : H) :
+  let ref_interpreter : '&mut (Interpreter.t WIRE WIRE_types) := make_ref 0 in
+  let ref_host : '&mut H := make_ref 1 in
+  {{
+    SimulateM.eval_f
+      (run_mload run_InterpreterTypes_for_WIRE ref_interpreter ref_host)
+      ([interpreter; _host]%stack) 🌲
+    (
+      Output.Success tt,
+      [
+        mload interpreter;
+        _host
+      ]%stack
+    )
+  }}.
+Proof.
+  intros.
+  unfold mload.
+  gas_macro_eq InterpreterTypesEq.
+  popn_top_macro_eq InterpreterTypesEq.
+  as_usize_or_fail_macro_eq InterpreterTypesEq.
+  resize_memory_macro_eq InterpreterTypesEq.
+  s. {
+    apply InterpreterTypesEq.
+  }
+  s. {
+    apply InterpreterTypesEq.
+  }
+  s. {
+    s_apply Impl_Uint.try_from_be_slice_eq.
+  }
+  s. {
+    apply Impl_Option.unwrap_eq.
+    admit.
+  }
+  s.
+Admitted.
