RocqOfRust/revm/revm_interpreter/instructions/simulate/memory/mstore.v
@@ -1,0 +1,91 @@
+Require Import simulate.RocqOfRust.
+Require Import alloy_primitives.links.aliases.
+Require Import core.links.array.
+Require Import core.ops.simulate.deref.
+Require Import core.simulate.array.
+Require Import core.simulate.option.
+Require Import revm.revm_context_interface.links.host.
+Require Import revm.revm_interpreter.gas.simulate.constants.
+Require Import revm.revm_interpreter.instructions.links.memory.mstore.
+Require Import revm.revm_interpreter.instructions.simulate.macros.
+Require Import revm.revm_interpreter.interpreter.simulate.shared_memory.
+Require Import revm.revm_interpreter.links.gas.
+Require Import revm.revm_interpreter.links.interpreter.
+Require Import revm.revm_interpreter.links.interpreter_types.
+Require Import revm.revm_interpreter.simulate.gas.
+Require Import revm.revm_interpreter.simulate.interpreter_types.
+Require Import revm.revm_specification.links.hardfork.
+Require Import revm.revm_specification.simulate.hardfork.
+Require Import ruint.links.lib.
+Require Import ruint.simulate.bytes.
+Require Import ruint.simulate.from.
+Require Import ruint.simulate.lib.
+
+Definition mstore
+    {WIRE : Set} `{Link WIRE}
+    {WIRE_types : InterpreterTypes.Types.t} `{InterpreterTypes.Types.AreLinks WIRE_types}
+    `{IInterpreterTypes : !InterpreterTypes.C WIRE_types}
+    (interpreter : Interpreter.t WIRE WIRE_types) :
+    Interpreter.t WIRE WIRE_types :=
+  gas_macro interpreter constants.VERYLOW id (fun interpreter =>
+  popn_macro interpreter 2 id (fun arr interpreter =>
+  let '⟬ offset; value ⟭ := arr.(array.value) in
+  as_usize_or_fail_ret_macro interpreter offset None id (fun offset interpreter =>
+  resize_memory_macro interpreter offset 32 id (fun interpreter =>
+  let memory :=
+    IInterpreterTypes.(InterpreterTypes.MemoryTrait_for_Memory).(MemoryTrait.set)
+      interpreter.(Interpreter.memory)
+      offset
+      (ArrayPairs.to_list (Impl_Uint.to_be_bytes value).(array.value)) in
+  interpreter <| Interpreter.memory := memory |>
+  )))).
+
+Lemma mstore_eq
+    {WIRE H : Set} `{Link WIRE} `{Link H}
+    {WIRE_types : InterpreterTypes.Types.t} `{InterpreterTypes.Types.AreLinks WIRE_types}
+    {H_types : Host.Types.t} `{Host.Types.AreLinks H_types}
+    (run_InterpreterTypes_for_WIRE : InterpreterTypes.Run WIRE WIRE_types)
+    (IInterpreterTypes : InterpreterTypes.C WIRE_types)
+    (InterpreterTypesEq :
+      InterpreterTypes.Eq.t WIRE WIRE_types run_InterpreterTypes_for_WIRE IInterpreterTypes)
+    (interpreter : Interpreter.t WIRE WIRE_types)
+    (_host : H) :
+  let ref_interpreter : '&mut (Interpreter.t WIRE WIRE_types) := make_ref 0 in
+  let ref_host : '&mut H := make_ref 1 in
+  {{
+    SimulateM.eval_f
+      (run_mstore run_InterpreterTypes_for_WIRE ref_interpreter ref_host)
+      ([interpreter; _host]%stack) 🌲
+    (
+      Output.Success tt,
+      [
+        mstore interpreter;
+        _host
+      ]%stack
+    )
+  }}.
+Proof.
+  intros.
+  with_strategy transparent [run_mstore] unfold mstore, run_mstore; cbn.
+  gas_macro_eq InterpreterTypesEq.
+  popn_macro_eq InterpreterTypesEq.
+  match goal with
+  | array : array.t aliases.U256.t _ |- _ =>
+    destruct array as [[offset [value []]]]
+  end.
+  as_usize_or_fail_macro_eq InterpreterTypesEq.
+  resize_memory_macro_eq InterpreterTypesEq.
+  s. {
+    s_apply Impl_Uint.to_be_bytes_eq.
+  }
+  s. {
+    set (ref_array := Ref.cast_to _ _).
+    eapply (array.pointer_coercion_unsize_array_to_slice_eq ref_array _);
+      repeat unshelve econstructor.
+  }
+  s. {
+    apply InterpreterTypesEq.
+  }
+  s.
+  now destruct IInterpreterTypes.(InterpreterTypes.MemoryTrait_for_Memory).(MemoryTrait.resize).
+Qed.
