RocqOfRust/revm/revm_interpreter/instructions/simulate/system/gas.v
@@ -2,8 +2,10 @@ Require Import simulate.RocqOfRust.
 Require Import revm.revm_interpreter.gas.simulate.constants.
 Require Import revm.revm_interpreter.instructions.links.system.gas.
 Require Import revm.revm_interpreter.instructions.simulate.macros.
+Require Import revm.revm_interpreter.links.gas.
 Require Import revm.revm_interpreter.links.interpreter.
 Require Import revm.revm_interpreter.links.interpreter_types.
+Require Import revm.revm_interpreter.simulate.interpreter_types.
 Require Import ruint.links.lib.
 
 Definition gas
