RocqOfRust/revm/revm_interpreter/instructions/simulate/system/keccak256.v
@@ -5,6 +5,7 @@ Require Import revm.revm_interpreter.instructions.links.system.keccak256.
 Require Import revm.revm_interpreter.instructions.simulate.macros.
 Require Import revm.revm_interpreter.links.interpreter.
 Require Import revm.revm_interpreter.links.interpreter_types.
+Require Import revm.revm_interpreter.simulate.interpreter_types.
 Require Import ruint.links.lib.
 
 Definition keccak256
