RocqOfRust/revm/revm_interpreter/instructions/simulate/system/returndatacopy.v
@@ -4,6 +4,7 @@ Require Import revm.revm_interpreter.instructions.simulate.macros.
 Require Import revm.revm_specification.links.hardfork.
 Require Import revm.revm_interpreter.links.interpreter.
 Require Import revm.revm_interpreter.links.interpreter_types.
+Require Import revm.revm_interpreter.simulate.interpreter_types.
 
 Definition returndatacopy
     {WIRE : Set} `{Link WIRE}
