RocqOfRust/ruint/simulate/pow.v
@@ -1,0 +1,22 @@
+Require Import simulate.RocqOfRust.
+Require Import ruint.links.pow.
+
+Module Impl_Uint.
+  Definition pow {BITS LIMBS : usize} (base exp : lib.Uint.t BITS LIMBS) :
+      lib.Uint.t BITS LIMBS :=
+    {| lib.Uint.value := (base.(lib.Uint.value) ^ exp.(lib.Uint.value)) mod (2 ^ BITS.(Integer.value)) |}.
+
+  Lemma pow_eq
+      (stack : Stack.t)
+      (BITS LIMBS : usize) (base exp : lib.Uint.t BITS LIMBS) :
+    {{
+      SimulateM.eval_f
+        (Impl_Uint.run_pow BITS LIMBS base exp)
+        stack 🌲
+      (
+        Output.Success (pow base exp),
+        stack
+      )
+    }}.
+  Admitted.
+End Impl_Uint.
